v2/order.v
@@ -15,6 +15,30 @@ Record Group_Order (ord : positive) := Group_Enumeration {
   enum_surj : ∀ π, Generates π -> ∃ i, i ≤ ord ∧ π ≡ enum i;
 }.
 
+Lemma generates_e :
+  Generates ∅.
+Proof.
+exists []; split; [|done].
+apply list_subseteq_nil.
+Qed.
+
+Lemma generates_generator σ :
+  σ ∈ gen -> Generates σ.
+Proof.
+exists [σ]; split.
+- intros a Ha; decompose_elem_of_list; subst; done.
+- symmetry; apply (right_id ∅ (⋅)).
+Qed.
+
+Lemma generates_compose τ π :
+  Generates τ -> Generates π -> Generates (π⋅τ).
+Proof.
+intros [w_τ [H1 H2]] [w_π [H3 H4]]; exists (w_π ++ w_τ); split.
+- intros a Ha; apply elem_of_app in Ha; firstorder.
+- rewrite H2, H4; clear; induction w_π; cbn; intros.
+  apply (left_id ∅ (⋅)). rewrite <-(assoc (⋅)), IHw_π; done.
+Qed.
+
 End Generating_set.
 
 Lemma unit_group_order :
